syntax and some small step

theories/lang.v
@@ -1,3 +1,211 @@
-Inductive foo :=
-  | Bar
+From stdpp Require Export binders strings.
+From l3 Require Export loclit.
+From Autosubst Require Export Autosubst.
+From iris.proofmode Require Import proofmode.
+
+Declare Scope expr_scope.
+Declare Scope val_scope.
+Delimit Scope expr_scope with E.
+Delimit Scope val_scope with V.
+
+(* This is structured such that it is possible to instantiate Iris using this
+   language (even though our wp might be specialized to just this language) *)
+(* The structure of this file follows HeapLang closely:
+   https://gitlab.mpi-sws.org/iris/iris/-/blob/master/iris_heap_lang/lang.v *)
+
+Module l3_lang.
+
+(* Step 1: syntax of expressions and values *)
+
+(* https://www.ccs.neu.edu/home/amal/papers/linloc-fi07.pdf *)
+(* See Section 3.1 *)
+
+Inductive loc :=
+  (* Using Autosubset and DeBrujin indices for location variables η *)
+  | LocVar (ρ : var)
+  | LocConst (l : loclit)
 .
+
+Inductive expr :=
+  (* Lets us include values directly, even with some redundancy.
+     Expression versions of values step to Val, just like in HeapLang *)
+  | Val (v : val)
+  (* HeapLang does not duplicate literals but does duplicate things
+     like Lam, which need to be an expr in order to be substituted into.
+     Pair also needs to be an expr, since the value form is different.
+     The "expr" versions of `val`s will step to the corresponding value.
+     *)
+  (* | Unit : expr *)
+  | LetUnit (e1 e2 : expr)
+  | Pair (e1 e2 : expr)
+  | LetPair (x1 x2 : binder) (e1 e2 : expr)
+  (* Using stdpp binders for program variables x *)
+  | Var (x : binder)
+  | Lam (x : binder) (e : expr)
+  | App (e1 e2 : expr)
+  (* | Bang (v : val) *)
+  | LetBang (x : binder) (e1 e2 : expr)
+  | Dup (e : expr)
+  | Drp (e : expr)
+  (* | Ptr (l : loclit) *)
+  (* | Cap : expr *)
+  | New (e : expr)
+  | Free (e : expr)
+  | Swap (e1 e2 e3 : expr)
+  (* Λη.e *)
+  | LocLam (e : {bind loc in expr})
+  | LocApp (e : expr) (η : loc)
+  | LocPack (η : loc) (e : expr)
+  (* let ⌜ρ, x⌝ = e1 in e2 *)
+  | LocUnpack (x : binder) (e1 : expr) (e2 : {bind loc in expr})
+with val :=
+  | UnitV : val
+  | PairV (v1 v2 : val)
+  (* unlike L3, x is not a value *)
+  | LamV (x : binder) (e : expr)
+  | BangV (v : val)
+  | PtrV (l : loclit)
+  | CapV : val
+  | LocLamV (e : {bind loc in expr})
+  | LocPackV (η : loc) (e : expr)
+.
+
+Bind Scope expr_scope with expr.
+Bind Scope val_scope with val.
+
+(* Step 2: value and expr conversion functions *)
+
+Notation of_val := Val (only parsing).
+
+Definition to_val (e : expr) : option val :=
+  match e with
+  | Val v => Some v
+  | _ => None
+  end.
+
+
+(* The following lemmas are for "Equality and other typeclass stuff" *)
+(* The bodies of these lemmas are from HeapLang, mostly *)
+(* Not sure why these are needed but I bet they will come up... *)
+
+Lemma to_of_val v : to_val (of_val v) = Some v.
+Proof. by destruct v. Qed.
+
+Lemma of_to_val e v : to_val e = Some v → of_val v = e.
+Proof. destruct e=>//=. by intros [= <-]. Qed.
+
+Global Instance of_val_inj : Inj (=) (=) of_val.
+Proof. intros ??. congruence. Qed.
+
+(* in case we need these: *)
+(* Global Instance val_inhabited : Inhabited val := populate UnitV. *)
+(* Global Instance expr_inhabited : Inhabited expr := populate (Val inhabitant). *)
+
+(* May need EqDecision instances for expr and val *)
+
+(* Step 3: define semantics *)
+
+(* SimpLang suggests that we wrap this, so I am! *)
+Record store : Type := {
+  heap: gmap loclit val;
+}.
+
+(** the language interface needs these things to be inhabited, I believe *)
+Global Instance store_inhabited : Inhabited store :=
+  populate {| heap := inhabitant; |}.
+
+Definition state_upd_heap (f : gmap loclit val → gmap loclit val) (σ : store) : store :=
+  {| heap := f σ.(heap) |}.
+Global Arguments state_upd_heap _ !_ /.
+
+(* We need to talk about substitution in our semantics.
+   We follow HeapLang: substitution is _not_ capture-avoiding;
+   we do not substitute into values;
+   we work with appropriately closed things. *)
+
+Fixpoint subst_val (x : string) (v : val) (e : expr) :=
+  match e with
+  | Val _ => e
+  | LetUnit e1 e2 => LetUnit (subst_val x v e1) (subst_val x v e2)
+  | Pair e1 e2 => Pair (subst_val x v e1) (subst_val x v e2)
+  | LetPair x1 x2 e1 e2 => 
+    let e2' := if decide (BNamed x ≠ x1 ∧ BNamed x ≠ x2) 
+               then subst_val x v e2 else e2 in
+    LetPair x1 x2 (subst_val x v e1) e2'
+  | Var y => if decide (BNamed x = y) then Val v else Var y
+  | Lam y e => Lam y $ if decide (BNamed x ≠ y) then subst_val x v e else e
+  | App e1 e2 => App (subst_val x v e1) (subst_val x v e2)
+  | LetBang y e1 e2 =>
+    let e2' := if decide (BNamed x ≠ y) then subst_val x v e2 else e2 in
+    LetBang y (subst_val x v e1) e2'
+  | Dup e => Dup $ subst_val x v e
+  | Drp e => Drp $ subst_val x v e
+  | New e => New $ subst_val x v e
+  | Free e => Free $ subst_val x v e
+  | Swap e1 e2 e3 => 
+    Swap (subst_val x v e1) (subst_val x v e2) (subst_val x v e3)
+  | LocLam e => LocLam $ subst_val x v e
+  | LocApp e η => LocApp (subst_val x v e) η
+  | LocPack η e => LocPack η $ subst_val x v e
+  | LocUnpack y e1 e2 => 
+    let e2' := if decide (BNamed x ≠ y) then subst_val x v e2 else e2 in
+    LocUnpack y (subst_val x v e1) e2'
+  end.
+
+Definition subst_val' (mx : binder) (v : val) : expr → expr :=
+  match mx with BNamed x => subst_val x v | BAnon => id end.
+
+
+(* we also have to be able to substitute away location variables,
+   which we use the Autosubst machinery for! *)
+
+
+Inductive base_step : store * expr → store * expr → Prop :=
+  | SLetUnit σ e :
+    base_step (σ, LetUnit (Val UnitV) e) (σ, e)
+  (* Extra instruction needed to step a pairs of values into a
+     value which is a pair. See comments above for justification *)
+  | SPair σ v1 v2 :
+    base_step (σ, Pair (Val v1) (Val v2)) (σ, Val $ PairV v1 v2)
+  | SLetPair σ x1 x2 v1 v2 e e' :
+    e' = subst_val' x2 v2 (subst_val' x1 v1 e) →
+    base_step (σ, LetPair x1 x2 (Val $ PairV v1 v2) e) (σ, e')
+  | SLam σ x e :
+    base_step (σ, Lam x e) (σ, Val $ LamV x e)
+  | SApp σ x e v e' :
+    e' = subst_val' x v e →
+    base_step (σ, App (Val $ LamV x e) (Val v)) (σ, e')
+  | SLetBang σ x v e e' :
+    e' = subst_val' x v e →
+    base_step (σ, LetBang x (Val v) e) (σ, e')
+  | SDup σ v :
+    base_step (σ, Dup $ Val $ BangV v) (σ, Val $ PairV (BangV v) (BangV v))
+  | SDrp σ v :
+    base_step (σ, Drp $ Val $ BangV v) (σ, Val UnitV)
+  | SNew σ v (l : loclit) :
+    σ.(heap) !! l = None →
+    base_step 
+      (σ, New $ Val v)
+      (state_upd_heap <[l := v]> σ, 
+       (* ⌜l, (cap, !ptr v)⌝, plus awkward val wrapping *)
+       (* TODO: maybe the val wrapping is a little wrong here?? *)
+       Val $ LocPackV (LocConst l) $ Val $ PairV CapV $ BangV $ PtrV l)
+  | SFree σ l v :
+    σ.(heap) !! l = Some v →
+    base_step 
+      (σ, Free $ Val $ LocPackV (LocConst l) $ Val $ PairV CapV $ BangV $ PtrV l)
+      (state_upd_heap (delete l) σ, Val $ LocPackV (LocConst l) $ Val v)
+  | SSwap σ l v1 v2 :
+    σ.(heap) !! l = Some v1 →
+    base_step (σ, Swap (Val CapV) (Val $ PtrV l) (Val v2))
+              (state_upd_heap <[l := v2]> σ, Val $ PairV CapV v1)
+  | SLocLam σ e :
+    base_step (σ, LocLam e) (σ, Val $ LocLamV e)
+  (* app lam goes here *)
+  | SLocPack σ η e :
+    base_step (σ, LocPack η e) (σ, Val $ LocPackV η e)
+  (* pack unpack goes here *)
+.
+
+
+End l3_lang.
